Start to add typing for pure lists
Lists are represented using the usual encoding in terms of pairs and sums.
However, the typing rules need to be adjusted to preclude doing struct stores
with list types, because their dynamic size means the usual flattening of pairs
does not do the right thing.

These are purely for specifications, they're not intended to be the target
of any real Goose translation.

src/goose_lang/logical_reln_defns.v
@@ -125,6 +125,29 @@ Definition prodT_interp (t1 t2: sty) val_interp : sval → ival → iProp Σ :=
                    ∗ val_interp t1 vs1 v1
                    ∗ val_interp t2 vs2 v2)%I.
 
+Fixpoint listT_interp_aux (val_interp : sval → ival → iProp Σ)
+         (lvs : list sval) (lv : list ival) : iProp Σ :=
+  (match lvs, lv with
+  | nil, nil => True%I
+  | vs :: lvs, v :: lv =>
+    val_interp vs v ∗ listT_interp_aux val_interp lvs lv
+  | _, _ => False%I
+  end)%I.
+
+Fixpoint listEnc {EXT : ext_op} (l: list (@val EXT)) : @val EXT :=
+  match l with
+  | nil => InjLV (LitV LitUnit)
+  | v :: l => InjRV (PairV v (listEnc l))
+  end.
+
+Definition listT_interp (t: sty) (val_interp : sty → sval → ival → iProp Σ) : sval → ival → iProp Σ :=
+  λ vs v, (∃ lvs lv, ⌜ vs = listEnc lvs ∧ v = listEnc lv ⌝ ∗ listT_interp_aux (val_interp t) lvs lv)%I.
+
+(*
+Definition listT_interp (t: sty) (val_list_interp : sty → list sval → list ival → iProp Σ) : sval → ival → iProp Σ :=
+  λ vs v, (∃ lvs lv, ⌜ vs = listEnc lvs ∧ v = listEnc lv ⌝ ∗ val_list_interp t lvs lv)%I.
+*)
+
 Definition sumT_interp (t1 t2: sty) val_interp : sval → ival → iProp Σ :=
   λ vs v, ((∃ v' vs', ⌜ v = InjLV v' ∧
                                 vs = InjLV vs'⌝
@@ -175,6 +198,7 @@ Fixpoint val_interp (t: sty) {struct t} :=
   match t with
   | baseT bt => base_ty_interp bt
   | prodT t1 t2 => prodT_interp t1 t2 val_interp
+  | listT t => listT_interp t val_interp
   | sumT t1 t2 => sumT_interp t1 t2 val_interp
   | arrayT t => arrayT_interp t flatten_val_interp
   | arrowT t1 t2 => arrowT_interp t1 t2 val_interp
@@ -185,6 +209,7 @@ Fixpoint val_interp (t: sty) {struct t} :=
  flatten_val_interp (t: sty) {struct t} : list (sval → ival → iProp Σ) :=
     match t with
     | prodT t1 t2 => flatten_val_interp t1 ++ flatten_val_interp t2
+    | listT t => [listT_interp t val_interp]
     | baseT unitBT => []
     | baseT ty => [base_ty_interp ty]
     | sumT t1 t2 => [sumT_interp t1 t2 val_interp]
@@ -296,6 +321,22 @@ Definition ctx_has_semTy `{hG: !heapG Σ} `{hRG: !refinement_heapG Σ} {hS: styG
 Global Instance base_interp_pers Σ es e t:
       Persistent (base_ty_interp (Σ := Σ) t es e).
 Proof. destruct t; apply _. Qed.
+
+Instance listT_interp_aux_pers `{hG: !heapG Σ} `{hRG: !refinement_heapG Σ} ls l
+       (vTy: sval → ival → iProp Σ) :
+       (∀ es' e', Persistent (vTy es' e')) →
+       Persistent (listT_interp_aux vTy ls l).
+Proof.
+  intros ?. revert l. induction ls; destruct l => //=; apply _.
+Qed.
+
+Instance listT_interp_pers `{hG: !heapG Σ} `{hRG: !refinement_heapG Σ} {hS: styG Σ} es e t
+       (vTy: sty → sval → ival → iProp Σ) :
+       (∀ t' es' e', Persistent (vTy t' es' e')) →
+       Persistent (listT_interp t vTy es e).
+Proof.
+  intros. rewrite /listT_interp. apply _.
+Qed.
 
 Global Instance val_interp_pers `{hG: !heapG Σ} `{hRG: !refinement_heapG Σ} {hS: styG Σ} es e t:
       Persistent (val_interp (hS := hS) t es e).
